refactor: split TM_Hoare.thy (2/2)
move Hoare related defs and lemmas from Computability.thy (previously TM_Hoare.thy) to TM_Hoare.thy (depends on Computability.thy)

swap def/altdef for definitions that use Hoare defs but have simple alternatives

Computability.thy
@@ -1,4 +1,4 @@
-theory TM_Hoare (* TODO find better name. maybe "TM_Computation" *)
+theory Computability
   imports TM
 begin
 
@@ -123,76 +123,6 @@ using assms unfolding run_def by (fact final_mono)
 end \<comment> \<open>\<^locale>\<open>TM\<close>\<close>
 
 
-subsection \<open>Hoare Rules\<close>
-
-type_synonym ('q, 's) assert = "('q, 's) TM_config \<Rightarrow> bool"
-
-definition hoare_halt :: "('q, 's) assert \<Rightarrow> ('q, 's) TM \<Rightarrow> ('q, 's) assert \<Rightarrow> bool"
-  where "hoare_halt P M Q \<equiv>
-    (\<forall>c. P c \<longrightarrow> (\<exists>n. let cn = TM.steps M n c in TM.is_final M cn \<and> Q cn))"
-
-lemma hoare_haltI[intro]:
-  fixes P Q
-  assumes "\<And>c. P c \<Longrightarrow> \<exists>n. TM.is_final M (TM.steps M n c) \<and> Q (TM.steps M n c)"
-  shows "hoare_halt P M Q"
-  unfolding hoare_halt_def Let_def using assms by blast
-
-lemma hoare_haltE[elim]:
-  fixes c
-  assumes "hoare_halt P M Q"
-    and "P c"
-  obtains n where "TM.is_final M (TM.steps M n c)" and "Q (TM.steps M n c)"
-  using assms
-  unfolding hoare_halt_def Let_def by blast
-
-lemma hoare_haltE2[elim]:
-  fixes c
-  assumes "hoare_halt P M Q"
-    and "P c"
-  shows "\<exists>n. TM.is_final M (TM.steps M n c) \<and> Q (TM.steps M n c)"
-  using assms unfolding hoare_halt_def Let_def by blast
-
-lemma hoare_contr:
-  assumes "hoare_halt P M (\<lambda>_. False)" and "P c"
-  shows "False"
-  using assms by (rule hoare_haltE)
-
-lemma hoare_imp[elim]:
-  assumes "hoare_halt P M Q"
-    and P': "\<And>c. P' c \<Longrightarrow> P c"
-    and Q': "\<And>c. Q c \<Longrightarrow> Q' c"
-  shows "hoare_halt P' M Q'"
-proof (intro hoare_haltI)
-  fix c assume "P' c"
-  with P' and \<open>hoare_halt P M Q\<close> obtain n
-    where f: "TM.is_final M (TM.steps M n c)" and Q: "Q (TM.steps M n c)" by blast
-  with Q' show "\<exists>n. TM.is_final M (TM.steps M n c) \<and> Q' (TM.steps M n c)" by blast
-qed
-
-
-lemma hoare_true: "hoare_halt P M Q \<Longrightarrow> hoare_halt P M (\<lambda>_. True)" by fast
-
-lemma hoare_and[intro]:
-  assumes h1: "hoare_halt P M Q1"
-    and h2: "hoare_halt P M Q2"
-  shows "hoare_halt P M (\<lambda>c. Q1 c \<and> Q2 c)"
-proof
-  fix c assume "P c"
-  from h1 and \<open>P c\<close> obtain n1
-    where fn1: "TM.is_final M (TM.steps M n1 c)" and q1: "Q1 (TM.steps M n1 c)" by (rule hoare_haltE)
-  from h2 and \<open>P c\<close> obtain n2
-    where fn2: "TM.is_final M (TM.steps M n2 c)" and q2: "Q2 (TM.steps M n2 c)" by (rule hoare_haltE)
-
-  define n::nat where "n \<equiv> max n1 n2"
-  hence "n1 \<le> n" "n2 \<le> n" by simp+
-  let ?cn = "TM.steps M n c"
-  from fn1 and \<open>n1 \<le> n\<close> have steps1: "?cn = TM.steps M n1 c" by (fact TM.final_le_steps)
-  from fn2 and \<open>n2 \<le> n\<close> have steps2: "?cn = TM.steps M n2 c" by (fact TM.final_le_steps)
-  from fn1 q1 q2 have "TM.is_final M ?cn \<and> Q1 ?cn \<and> Q2 ?cn" by (fold steps1 steps2) blast
-  then show "\<exists>n. TM.is_final M (TM.steps M n c) \<and> Q1 (TM.steps M n c) \<and> Q2 (TM.steps M n c)" ..
-qed
-
-
 definition (in TM) "on_input w \<equiv> (\<lambda>c. c = initial_config w)"
 
 lemma on_inputI[intro, simp]: "TM.on_input M w (TM.initial_config M w)"
@@ -200,60 +130,29 @@ lemma on_inputI[intro, simp]: "TM.on_input M w (TM.initial_config M w)"
 
 
 definition (in TM) halts_config :: "('q, 's) TM_config \<Rightarrow> bool"
-  where "halts_config c \<equiv> hoare_halt (\<lambda>x. x = c) M (\<lambda>_. True)"
+  where "halts_config c \<equiv> \<exists>n. is_final (steps n c)"
 
-lemma halts_config_altdef: "TM.halts_config M c \<longleftrightarrow> (\<exists>n. TM.is_final M (TM.steps M n c))"
-  unfolding TM.halts_config_def by fast
-
-mk_ide (in -) halts_config_altdef |intro halts_confI[intro]| |dest halts_confD[dest]|
-
-
-lemma (in TM) hoare_halt_init_conf:
-  "hoare_halt (TM.on_input M w) M P \<longleftrightarrow> (\<exists>n. let cn = run n w in is_final cn \<and> P cn)"
-  unfolding hoare_halt_def TM.on_input_def run_def by blast
+mk_ide (in -) TM.halts_config_def |intro halts_confI[intro]| |dest halts_confD[dest]|
 
 
 definition (in TM) halts :: "'s list \<Rightarrow> bool"
   where "halts w \<equiv> halts_config (initial_config w)"
 declare TM.halts_def[simp]
 
-lemma halts_altdef: "TM.halts M w \<longleftrightarrow> hoare_halt (TM.on_input M w) M (\<lambda>_. True)"
-  unfolding TM.halts_def TM.halts_config_def TM.on_input_def ..
-
 lemma halts_altdef2: "TM.halts M w \<longleftrightarrow> (\<exists>n. TM.is_final M (TM.run M n w))"
-  by (simp add: TM.run_def halts_config_altdef)
+  by (simp add: TM.run_def TM.halts_config_def)
 
 
 lemma haltsI[intro]:
   assumes "\<exists>n. TM.is_final M (TM.run M n w)"
   shows "TM.halts M w"
-  using assms by (simp add: TM.run_def halts_config_altdef)
+  using assms by (simp add: TM.run_def TM.halts_config_def)
 
 lemma haltsD[dest]: "TM.halts M w \<Longrightarrow> \<exists>n. TM.is_final M (TM.run M n w)"
   unfolding TM.halts_def TM.run_def by blast
 
 
-lemma hoare_halt_neg:
-  assumes "\<not> hoare_halt (TM.on_input M w) M Q"
-    and "TM.halts M w"
-  shows "hoare_halt (TM.on_input M w) M (\<lambda>tp. \<not> Q tp)"
-  using assms unfolding hoare_halt_def TM.halts_def Let_def TM.on_input_def by fast
-
-lemma halt_inj:
-  assumes "hoare_halt (TM.on_input M w) M (\<lambda>c. f c = x)"
-      and "hoare_halt (TM.on_input M w) M (\<lambda>c. f c = y)"
-    shows "x = y"
-proof (rule ccontr)
-  assume "x \<noteq> y"
-  then have *: "a = x \<and> a = y \<longleftrightarrow> False" for a by blast
-
-  from assms have "hoare_halt (TM.on_input M w) M (\<lambda>c. f c = x \<and> f c = y)" by (rule hoare_and)
-  then have "hoare_halt (TM.on_input M w) M (\<lambda>_. False)" unfolding * .
-  then show False by blast
-qed
-
-
-subsection\<open>Output\<close>
+subsubsection\<open>Output\<close>
 
 context TM
 begin
@@ -283,25 +182,13 @@ lemma clean_outputD[dest]: "clean_output c \<Longrightarrow> output_of c = w \<L
 lemma clean_output_alt: "clean_output c \<and> output_of c = w \<longleftrightarrow> last (tapes c) = <w>\<^sub>t\<^sub>p"
   unfolding clean_output_def by force
 
+end \<comment> \<open>context \<^locale>\<open>TM\<close>\<close>
 
-(* TODO document, clean up *)
 
-definition (in -) [simp]: "hoare_run w M P \<equiv> hoare_halt (TM.on_input M w) M P"
+subsubsection\<open>Execution Time\<close>
 
-definition "computes_word w w' \<equiv> hoare_run w M (\<lambda>c. clean_output c \<and> output_of c = w')"
-
-definition "computes f \<equiv> \<forall>w. computes_word w (f w)"
-declare (in -) TM.computes_def[simp]
-
-lemma hoare_run_halts[dest]: "hoare_run w M P \<Longrightarrow> halts w"
-  unfolding halts_altdef hoare_run_def by (rule hoare_true)
-
-lemma computes_word_halts[dest]: "computes_word w w' \<Longrightarrow> halts w"
-  unfolding computes_word_def by (rule hoare_run_halts)
-
-lemma computes_halts[dest]: "computes f \<Longrightarrow> halts w"
-  unfolding halts_altdef2 by auto
-
+context TM
+begin
 
 definition "config_time c \<equiv> LEAST n. is_final (steps n c)"
 
@@ -322,7 +209,7 @@ lemma conf_time_geD[dest, elim]:
   shows "is_final (steps n c)"
 proof -
   from assms(2) have "is_final (steps (LEAST n. is_final (steps n c)) c)"
-    unfolding halts_config_altdef by (rule LeastI_ex)
+    unfolding halts_config_def by (rule LeastI_ex)
   with assms(1) show ?thesis unfolding config_time_def by blast
 qed
 
@@ -383,48 +270,6 @@ lemma final_run_time[intro]: "is_final (run n w) \<Longrightarrow> run n w = com
 corollary halts_compute_final[dest]: "halts w \<Longrightarrow> is_final (compute w)"
   unfolding run_def halts_def time_def by (fact conf_time_finalI)
 
-lemma hoare_run_altdef: "hoare_run w M P \<longleftrightarrow> halts w \<and> P (compute w)"
-proof (rule iffI)
-  assume "hoare_run w M P"
-  then have "\<exists>n. let cn = run n w in is_final cn \<and> P cn"
-    unfolding hoare_run_def hoare_halt_init_conf .
-  then obtain n where "is_final (run n w)" and "P (run n w)" unfolding Let_def by blast
-  then show "halts w \<and> P (compute w)" using computeI by blast
-next
-  assume "halts w \<and> P (compute w)"
-  then have "halts w" and "P (compute w)" by blast+
-  from \<open>halts w\<close> have "is_final (compute w)" by blast
-  with \<open>P (compute w)\<close> show "hoare_run w M P"
-    unfolding hoare_run_def hoare_halt_init_conf Let_def by blast
-qed
-
-lemma hoare_run_run[dest]: "hoare_run w M P \<Longrightarrow> P (compute w)" unfolding hoare_run_altdef by blast
-
-lemma run_hoare_run[simp]: "halts w \<Longrightarrow> hoare_run w M P = P (compute w)"
-  unfolding hoare_run_altdef by blast
-
-
-lemma computes_word_output[dest]:
-  assumes "computes_word w w'"
-  shows "last (tapes (compute w)) = <w'>\<^sub>t\<^sub>p"
-proof -
-  let ?c = "run (time w) w"
-  from assms have "clean_output ?c" and "output_of ?c = w'" unfolding computes_word_def by blast+
-  then obtain x where "last (tapes ?c) = <x>\<^sub>t\<^sub>p" unfolding clean_output_def by blast
-  then have "output_of ?c = x" by blast
-  with \<open>output_of ?c = w'\<close> have "x = w'" by blast
-  with \<open>last (tapes ?c) = <x>\<^sub>t\<^sub>p\<close> show ?thesis by blast
-qed
-
-lemma computes_output: "computes f \<Longrightarrow> last (tapes (compute w)) = <f w>\<^sub>t\<^sub>p"
-  by (intro computes_word_output) simp
-
-lemma output_computes_word:
-  assumes "halts w"
-    and "last (tapes (compute w)) = <w'>\<^sub>t\<^sub>p"
-  shows "computes_word w w'"
-  unfolding computes_word_def run_hoare_run[OF \<open>halts w\<close>] clean_output_alt by (fact assms(2))
-
 
 lemma config_time_offset:
   fixes c0
@@ -472,10 +317,6 @@ next
   finally show ?thesis by presburger
 qed
 
-lemma computes_word_altdef: "computes_word w w' \<longleftrightarrow> halts w \<and> last (tapes (compute w)) = <w'>\<^sub>t\<^sub>p"
-  unfolding computes_word_def
-  using TM.clean_output_alt TM.hoare_run_altdef  by blast
-
 end \<comment> \<open>\<^locale>\<open>TM\<close>\<close>
 
 lemma config_time_eqI[intro]:
@@ -495,16 +336,6 @@ lemma time_eqI[intro]:
   shows "TM.time M1 w1 - n1 = TM.time M2 w2"
   using assms unfolding TM.time_def TM.run_def TM.halts_def by (fact config_time_eqI)
 
-locale Rej_TM = TM "rejecting_TM q0 s" for q0 :: 'q and s :: 's
-begin
-
-lemma M_rec: "M_rec = rejecting_TM_rec q0 s" using Abs_TM_inverse rejecting_TM_valid
-  unfolding rejecting_TM_def by fast
-lemmas M_fields = TM_fields_defs[unfolded M_rec rejecting_TM_rec_def TM_record.simps]
-lemmas [simp] = M_fields(1-6)
-
-lemma rej_tm_time: "time w = 0" by simp
-end
 
 subsection\<open>Deciding Languages\<close>
 context TM begin
@@ -554,6 +385,20 @@ qed
 lemma decides_altdef4: "decides_word L w \<longleftrightarrow> (if w \<in> L then accepts w else rejects w)"
   unfolding decides_def using acc_not_rej by (cases "w \<in> L") auto
 
+end
+
+
+(* TODO find a better place for the rejecting TM *)
+
+locale Rej_TM = TM "rejecting_TM q0 s" for q0 :: 'q and s :: 's
+begin
+
+lemma M_rec: "M_rec = rejecting_TM_rec q0 s" using Abs_TM_inverse rejecting_TM_valid
+  unfolding rejecting_TM_def by fast
+lemmas M_fields = TM_fields_defs[unfolded M_rec rejecting_TM_rec_def TM_record.simps]
+lemmas [simp] = M_fields(1-6)
+
+lemma rej_tm_time: "time w = 0" by simp
 end
 
 (* Note: having this much code commented out leads to errors when importing this theory sometimes.
