TM_Hoare.thy
@@ -1,0 +1,181 @@
+subsection \<open>Hoare Rules\<close>
+
+theory TM_Hoare
+  imports Computability
+begin
+
+
+type_synonym ('q, 's) assert = "('q, 's) TM_config \<Rightarrow> bool"
+
+definition hoare_halt :: "('q, 's) assert \<Rightarrow> ('q, 's) TM \<Rightarrow> ('q, 's) assert \<Rightarrow> bool"
+  where "hoare_halt P M Q \<equiv>
+    (\<forall>c. P c \<longrightarrow> (\<exists>n. let cn = TM.steps M n c in TM.is_final M cn \<and> Q cn))"
+
+lemma hoare_haltI[intro]:
+  fixes P Q
+  assumes "\<And>c. P c \<Longrightarrow> \<exists>n. TM.is_final M (TM.steps M n c) \<and> Q (TM.steps M n c)"
+  shows "hoare_halt P M Q"
+  unfolding hoare_halt_def Let_def using assms by blast
+
+lemma hoare_haltE[elim]:
+  fixes c
+  assumes "hoare_halt P M Q"
+    and "P c"
+  obtains n where "TM.is_final M (TM.steps M n c)" and "Q (TM.steps M n c)"
+  using assms
+  unfolding hoare_halt_def Let_def by blast
+
+lemma hoare_haltE2[elim]:
+  fixes c
+  assumes "hoare_halt P M Q"
+    and "P c"
+  shows "\<exists>n. TM.is_final M (TM.steps M n c) \<and> Q (TM.steps M n c)"
+  using assms unfolding hoare_halt_def Let_def by blast
+
+lemma hoare_contr:
+  assumes "hoare_halt P M (\<lambda>_. False)" and "P c"
+  shows "False"
+  using assms by (rule hoare_haltE)
+
+lemma hoare_imp[elim]:
+  assumes "hoare_halt P M Q"
+    and P': "\<And>c. P' c \<Longrightarrow> P c"
+    and Q': "\<And>c. Q c \<Longrightarrow> Q' c"
+  shows "hoare_halt P' M Q'"
+proof (intro hoare_haltI)
+  fix c assume "P' c"
+  with P' and \<open>hoare_halt P M Q\<close> obtain n
+    where f: "TM.is_final M (TM.steps M n c)" and Q: "Q (TM.steps M n c)" by blast
+  with Q' show "\<exists>n. TM.is_final M (TM.steps M n c) \<and> Q' (TM.steps M n c)" by blast
+qed
+
+
+lemma hoare_true: "hoare_halt P M Q \<Longrightarrow> hoare_halt P M (\<lambda>_. True)" by fast
+
+lemma hoare_and[intro]:
+  assumes h1: "hoare_halt P M Q1"
+    and h2: "hoare_halt P M Q2"
+  shows "hoare_halt P M (\<lambda>c. Q1 c \<and> Q2 c)"
+proof
+  fix c assume "P c"
+  from h1 and \<open>P c\<close> obtain n1
+    where fn1: "TM.is_final M (TM.steps M n1 c)" and q1: "Q1 (TM.steps M n1 c)" by (rule hoare_haltE)
+  from h2 and \<open>P c\<close> obtain n2
+    where fn2: "TM.is_final M (TM.steps M n2 c)" and q2: "Q2 (TM.steps M n2 c)" by (rule hoare_haltE)
+
+  define n::nat where "n \<equiv> max n1 n2"
+  hence "n1 \<le> n" "n2 \<le> n" by simp+
+  let ?cn = "TM.steps M n c"
+  from fn1 and \<open>n1 \<le> n\<close> have steps1: "?cn = TM.steps M n1 c" by (fact TM.final_le_steps)
+  from fn2 and \<open>n2 \<le> n\<close> have steps2: "?cn = TM.steps M n2 c" by (fact TM.final_le_steps)
+  from fn1 q1 q2 have "TM.is_final M ?cn \<and> Q1 ?cn \<and> Q2 ?cn" by (fold steps1 steps2) blast
+  then show "\<exists>n. TM.is_final M (TM.steps M n c) \<and> Q1 (TM.steps M n c) \<and> Q2 (TM.steps M n c)" ..
+qed
+
+
+lemma halts_config_altdef: "TM.halts_config M c \<longleftrightarrow> hoare_halt (\<lambda>x. x = c) M (\<lambda>_. True)"
+  unfolding TM.halts_config_def by fast
+
+lemma (in TM) hoare_halt_init_conf:
+  "hoare_halt (TM.on_input M w) M P \<longleftrightarrow> (\<exists>n. let cn = run n w in is_final cn \<and> P cn)"
+  unfolding hoare_halt_def TM.on_input_def run_def by blast
+
+lemma halts_altdef: "TM.halts M w \<longleftrightarrow> hoare_halt (TM.on_input M w) M (\<lambda>_. True)"
+  unfolding TM.halts_def halts_config_altdef TM.on_input_def ..
+
+lemma hoare_halt_neg:
+  assumes "\<not> hoare_halt (TM.on_input M w) M Q"
+    and "TM.halts M w"
+  shows "hoare_halt (TM.on_input M w) M (\<lambda>tp. \<not> Q tp)"
+  using assms unfolding hoare_halt_def TM.halts_def Let_def TM.on_input_def by fast
+
+
+lemma halt_inj:
+  assumes "hoare_halt (TM.on_input M w) M (\<lambda>c. f c = x)"
+      and "hoare_halt (TM.on_input M w) M (\<lambda>c. f c = y)"
+    shows "x = y"
+proof (rule ccontr)
+  assume "x \<noteq> y"
+  then have *: "a = x \<and> a = y \<longleftrightarrow> False" for a by blast
+
+  from assms have "hoare_halt (TM.on_input M w) M (\<lambda>c. f c = x \<and> f c = y)" by (rule hoare_and)
+  then have "hoare_halt (TM.on_input M w) M (\<lambda>_. False)" unfolding * .
+  then show False by blast
+qed
+
+
+subsubsection\<open>Computes Predicate\<close>
+
+context TM
+begin
+
+(* TODO document, clean up *)
+
+definition (in -) [simp]: "hoare_run w M P \<equiv> hoare_halt (TM.on_input M w) M P"
+
+definition "computes_word w w' \<equiv> hoare_run w M (\<lambda>c. clean_output c \<and> output_of c = w')"
+
+
+lemma hoare_run_altdef: "hoare_run w M P \<longleftrightarrow> halts w \<and> P (compute w)"
+proof (rule iffI)
+  assume "hoare_run w M P"
+  then have "\<exists>n. let cn = run n w in is_final cn \<and> P cn"
+    unfolding hoare_run_def hoare_halt_init_conf .
+  then obtain n where "is_final (run n w)" and "P (run n w)" unfolding Let_def by blast
+  then show "halts w \<and> P (compute w)" using computeI by blast
+next
+  assume "halts w \<and> P (compute w)"
+  then have "halts w" and "P (compute w)" by blast+
+  from \<open>halts w\<close> have "is_final (compute w)" by blast
+  with \<open>P (compute w)\<close> show "hoare_run w M P"
+    unfolding hoare_run_def hoare_halt_init_conf Let_def by blast
+qed
+
+
+definition "computes f \<equiv> \<forall>w. computes_word w (f w)"
+declare (in -) TM.computes_def[simp]
+
+lemma hoare_run_halts[dest]: "hoare_run w M P \<Longrightarrow> halts w"
+  unfolding halts_altdef hoare_run_def by (rule hoare_true)
+
+lemma computes_word_halts[dest]: "computes_word w w' \<Longrightarrow> halts w"
+  unfolding computes_word_def by (rule hoare_run_halts)
+
+lemma computes_halts[dest]: "computes f \<Longrightarrow> halts w"
+  unfolding halts_altdef2 by auto
+
+
+lemma hoare_run_run[dest]: "hoare_run w M P \<Longrightarrow> P (compute w)" unfolding hoare_run_altdef by blast
+
+lemma run_hoare_run[simp]: "halts w \<Longrightarrow> hoare_run w M P = P (compute w)"
+  unfolding hoare_run_altdef by blast
+
+
+lemma computes_word_output[dest]:
+  assumes "computes_word w w'"
+  shows "last (tapes (compute w)) = <w'>\<^sub>t\<^sub>p"
+proof -
+  let ?c = "run (time w) w"
+  from assms have "clean_output ?c" and "output_of ?c = w'" unfolding computes_word_def by blast+
+  then obtain x where "last (tapes ?c) = <x>\<^sub>t\<^sub>p" unfolding clean_output_def by blast
+  then have "output_of ?c = x" by blast
+  with \<open>output_of ?c = w'\<close> have "x = w'" by blast
+  with \<open>last (tapes ?c) = <x>\<^sub>t\<^sub>p\<close> show ?thesis by blast
+qed
+
+lemma computes_output: "computes f \<Longrightarrow> last (tapes (compute w)) = <f w>\<^sub>t\<^sub>p"
+  by (intro computes_word_output) simp
+
+lemma output_computes_word:
+  assumes "halts w"
+    and "last (tapes (compute w)) = <w'>\<^sub>t\<^sub>p"
+  shows "computes_word w w'"
+  unfolding computes_word_def run_hoare_run[OF \<open>halts w\<close>] clean_output_alt by (fact assms(2))
+
+
+lemma computes_word_altdef: "computes_word w w' \<longleftrightarrow> halts w \<and> last (tapes (compute w)) = <w'>\<^sub>t\<^sub>p"
+  unfolding computes_word_def hoare_run_altdef by blast
+
+end \<comment> \<open>context \<^locale>\<open>TM\<close>\<close>
+
+end
